rocq/theories/TypeSystem/CheckerSoundness.v
@@ -138,6 +138,17 @@ Proof.
     f_equal. apply IH. exact HΩ.
 Qed.
 
+Lemma lifetime_list_eqb_true : forall l1 l2,
+  lifetime_list_eqb l1 l2 = true -> l1 = l2.
+Proof.
+  induction l1 as [|lt1 l1 IH]; intros l2 H.
+  - destruct l2; simpl in H; try discriminate; reflexivity.
+  - destruct l2 as [|lt2 l2]; simpl in H; try discriminate.
+    apply andb_true_iff in H as [Hlt Hrest].
+    apply lifetime_eqb_eq in Hlt. subst lt2.
+    f_equal. apply IH. exact Hrest.
+Qed.
+
 Lemma ty_depth_fn_arg_lt : forall u ts r t,
   In t ts -> ty_depth t < ty_depth (MkTy u (TFn ts r)).
 Proof.
@@ -183,14 +194,28 @@ Proof.
         (destruct u1, u2; simpl in Hu; try discriminate; reflexivity).
       subst u2.
       f_equal.
-      destruct c1 as [| | | | s1 | ts1 r1 | n1 Ω1 b1 | l1 k1 t1],
-               c2 as [| | | | s2 | ts2 r2 | n2 Ω2 b2 | l2 k2 t2];
+      destruct c1 as [| | | | s1 | i1 | name1 lts1 args1 | ts1 r1 | n1 Ω1 b1 | l1 k1 t1],
+               c2 as [| | | | s2 | i2 | name2 lts2 args2 | ts2 r2 | n2 Ω2 b2 | l2 k2 t2];
         simpl in Hc; try discriminate.
       + reflexivity.
       + reflexivity.
       + reflexivity.
       + reflexivity.
       + apply String.eqb_eq in Hc. subst. reflexivity.
+      + apply Nat.eqb_eq in Hc. subst. reflexivity.
+      + apply andb_true_iff in Hc as [Hname_lts Hargs].
+        apply andb_true_iff in Hname_lts as [Hname Hlts].
+        apply String.eqb_eq in Hname. subst name2.
+        apply lifetime_list_eqb_true in Hlts. subst lts2.
+        f_equal.
+        revert args2 Hlt Hargs.
+        induction args1 as [| t1 args1' IHargs]; intros args2 Hlt Hargs.
+        * destruct args2; [reflexivity | discriminate].
+        * destruct args2 as [| t2 args2']; [discriminate |].
+          simpl in Hargs. apply andb_true_iff in Hargs as [Ht Htail].
+          f_equal.
+          { apply IH; [simpl in Hlt; lia | exact Ht]. }
+          { apply IHargs; [simpl in *; lia | exact Htail]. }
       + apply andb_true_iff in Hc as [Hlist Hr].
         assert (Heqr : r1 = r2) by
           (apply IH; [pose proof (ty_depth_fn_ret_lt u1 ts1 r1); lia | exact Hr]).
@@ -227,14 +252,28 @@ Lemma ty_core_eqb_true : forall c1 c2,
   ty_core_eqb c1 c2 = true -> c1 = c2.
 Proof.
   intros c1 c2 H.
-  destruct c1 as [| | | | s1 | ts1 r1 | n1 Ω1 b1 | l1 k1 t1],
-           c2 as [| | | | s2 | ts2 r2 | n2 Ω2 b2 | l2 k2 t2];
+  destruct c1 as [| | | | s1 | i1 | name1 lts1 args1 | ts1 r1 | n1 Ω1 b1 | l1 k1 t1],
+           c2 as [| | | | s2 | i2 | name2 lts2 args2 | ts2 r2 | n2 Ω2 b2 | l2 k2 t2];
     simpl in H; try discriminate.
   - reflexivity.
   - reflexivity.
   - reflexivity.
   - reflexivity.
   - apply String.eqb_eq in H. subst. reflexivity.
+  - apply Nat.eqb_eq in H. subst. reflexivity.
+  - apply andb_true_iff in H as [Hname_lts Hargs].
+    apply andb_true_iff in Hname_lts as [Hname Hlts].
+    apply String.eqb_eq in Hname. subst name2.
+    apply lifetime_list_eqb_true in Hlts. subst lts2.
+    f_equal.
+    revert args2 Hargs.
+    induction args1 as [| t1 args1' IHargs]; intros args2 Hargs.
+    + destruct args2; [reflexivity | discriminate].
+    + destruct args2 as [| t2 args2']; [discriminate |].
+      simpl in Hargs. apply andb_true_iff in Hargs as [Ht Htail].
+      f_equal.
+      * apply ty_eqb_true. exact Ht.
+      * apply IHargs. exact Htail.
   - apply andb_true_iff in H as [Hlist Hr].
     assert (Heqr : r1 = r2) by (apply ty_eqb_true; exact Hr). subst r2.
     f_equal.
@@ -318,8 +357,8 @@ Proof.
   - simpl in H. discriminate.
   - destruct T_actual as [ua ca], T_expected as [ue ce].
     simpl in H. apply andb_true_iff in H as [Hu Hc].
-    destruct ca as [| | | | sa | tsa ra | na Ωa body_a | la rka Ta],
-             ce as [| | | | se | tse re | nb Ωb body_b | lb rkb Tb];
+    destruct ca as [| | | | sa | ia | struct_a ltsa argsa | tsa ra | na Ωa body_a | la rka Ta],
+             ce as [| | | | se | ie | struct_e ltse argse | tse re | nb Ωb body_b | lb rkb Tb];
       simpl in Hc; try discriminate;
       try (apply TC_Core;
            [apply usage_sub_bool_sound; exact Hu
@@ -352,14 +391,28 @@ Proof.
       * exact Hu.
       * exact Hnob.
       * eapply IH. exact Hrec.
-    + destruct Ωb as [|p Ωb]; [|discriminate].
-      apply andb_true_iff in Hc as [Hnob Hrec].
-      apply negb_true_iff in Hnob.
-      eapply ty_compatible_forall_generalize_unused_sound.
-      * exact Hu.
-      * exact Hnob.
-      * eapply IH. exact Hrec.
-    + apply andb_true_iff in Hc as [Hargs Hret].
+	    + destruct Ωb as [|p Ωb]; [|discriminate].
+	      apply andb_true_iff in Hc as [Hnob Hrec].
+	      apply negb_true_iff in Hnob.
+	      eapply ty_compatible_forall_generalize_unused_sound.
+	      * exact Hu.
+	      * exact Hnob.
+	      * eapply IH. exact Hrec.
+	    + destruct Ωb as [|p Ωb]; [|discriminate].
+	      apply andb_true_iff in Hc as [Hnob Hrec].
+	      apply negb_true_iff in Hnob.
+	      eapply ty_compatible_forall_generalize_unused_sound.
+	      * exact Hu.
+	      * exact Hnob.
+	      * eapply IH. exact Hrec.
+	    + destruct Ωb as [|p Ωb]; [|discriminate].
+	      apply andb_true_iff in Hc as [Hnob Hrec].
+	      apply negb_true_iff in Hnob.
+	      eapply ty_compatible_forall_generalize_unused_sound.
+	      * exact Hu.
+	      * exact Hnob.
+	      * eapply IH. exact Hrec.
+	    + apply andb_true_iff in Hc as [Hargs Hret].
       apply TC_Fn.
       * apply usage_sub_bool_sound. exact Hu.
       * eapply ty_compatible_args_contra_b_sound.
@@ -586,12 +639,14 @@ Proof.
         rewrite (ecall_collect_eq fenv Ω n l Γcallee) in Hinfer.
         rewrite Hcollect in Hinfer.
         destruct (ty_core Tcallee) eqn:Hcore.
-        * discriminate.
-        * discriminate.
-        * discriminate.
-        * discriminate.
-        * discriminate.
-        * destruct (check_arg_tys Ω arg_tys l0) as [err |] eqn:Hcheck; [discriminate |].
+	        * discriminate.
+	        * discriminate.
+	        * discriminate.
+	        * discriminate.
+	        * discriminate.
+	        * discriminate.
+	        * discriminate.
+	        * destruct (check_arg_tys Ω arg_tys l0) as [err |] eqn:Hcheck; [discriminate |].
           injection Hinfer as <- <-.
           eapply T_CallExpr_Fn.
           -- replace (MkTy (ty_usage Tcallee) (TFn l0 t)) with Tcallee.
