rocq/theories/TypeSystem/Program.v
@@ -1,0 +1,95 @@
+From Facet.TypeSystem Require Import Lifetime Types Syntax.
+From Stdlib Require Import List String Bool.
+Import ListNotations.
+
+(* ------------------------------------------------------------------ *)
+(* Top-level declarations for struct/trait planning                      *)
+(* ------------------------------------------------------------------ *)
+
+Record field_def : Type := MkFieldDef {
+  field_name       : string;
+  field_mutability : mutability;
+  field_ty         : Ty
+}.
+
+Record trait_bound : Type := MkTraitBound {
+  bound_type_index : nat;
+  bound_traits     : list string
+}.
+
+Record struct_def : Type := MkStructDef {
+  struct_name      : string;
+  struct_lifetimes : nat;
+  struct_type_params : nat;
+  struct_bounds    : list trait_bound;
+  struct_fields    : list field_def
+}.
+
+Record trait_def : Type := MkTraitDef {
+  trait_name        : string;
+  trait_type_params : nat;
+  trait_bounds      : list trait_bound
+}.
+
+Record impl_def : Type := MkImplDef {
+  impl_lifetimes    : nat;
+  impl_type_params  : nat;
+  impl_trait_name   : string;
+  impl_trait_args   : list Ty;
+  impl_for_ty       : Ty
+}.
+
+Record global_env : Type := MkGlobalEnv {
+  env_structs : list struct_def;
+  env_traits  : list trait_def;
+  env_impls   : list impl_def;
+  env_fns     : list fn_def
+}.
+
+Definition empty_global_env (fenv : list fn_def) : global_env :=
+  MkGlobalEnv [] [] [] fenv.
+
+Fixpoint lookup_struct_in (name : string) (structs : list struct_def) : option struct_def :=
+  match structs with
+  | [] => None
+  | s :: rest =>
+      if String.eqb name (struct_name s)
+      then Some s
+      else lookup_struct_in name rest
+  end.
+
+Definition lookup_struct (name : string) (env : global_env) : option struct_def :=
+  lookup_struct_in name (env_structs env).
+
+Fixpoint lookup_trait_in (name : string) (traits : list trait_def) : option trait_def :=
+  match traits with
+  | [] => None
+  | t :: rest =>
+      if String.eqb name (trait_name t)
+      then Some t
+      else lookup_trait_in name rest
+  end.
+
+Definition lookup_trait (name : string) (env : global_env) : option trait_def :=
+  lookup_trait_in name (env_traits env).
+
+Fixpoint lookup_impls_for_trait (name : string) (impls : list impl_def) : list impl_def :=
+  match impls with
+  | [] => []
+  | i :: rest =>
+      let rest' := lookup_impls_for_trait name rest in
+      if String.eqb name (impl_trait_name i) then i :: rest' else rest'
+  end.
+
+Definition usage_max_decl (u1 u2 : usage) : usage :=
+  match u1, u2 with
+  | ULinear, _ | _, ULinear => ULinear
+  | UAffine, _ | _, UAffine => UAffine
+  | UUnrestricted, UUnrestricted => UUnrestricted
+  end.
+
+Fixpoint usage_max_list (fields : list field_def) : usage :=
+  match fields with
+  | [] => UUnrestricted
+  | f :: rest => usage_max_decl (ty_usage (field_ty f)) (usage_max_list rest)
+  end.
